making Imp go fast with native registers

examples/tactics/Imp.fst
@@ -1,23 +1,19 @@
 module Imp
-
 //#set-options "--debug Imp --debug_level SMTQuery"
-
 open FStar.Mul
-open FStar.Tactics
-open CanonCommSemiring
-open FStar.Algebra.CommMonoid
+module R = Registers.List
 
-type rval = int
-type reg = | R of n:nat{n < 10}
-type regmap = reg -> rval
+type rval   = int
+type reg_t  = x:nat{x<=10}
+type regmap = R.regmap rval
 
 noeq
 type inst =
-    | Add : reg -> reg -> reg -> inst
-    | Sub : reg -> reg -> reg -> inst
-    | Mul : reg -> reg -> reg -> inst
-    | Const : rval -> reg -> inst
-    | If0 : reg -> prog -> prog -> inst
+    | Add : reg_t -> reg_t -> reg_t -> inst
+    | Sub : reg_t -> reg_t -> reg_t -> inst
+    | Mul : reg_t -> reg_t -> reg_t -> inst
+    | Const : rval -> reg_t -> inst
+    | If0 : reg_t -> prog -> prog -> inst
     | Seq : prog -> inst
 and prog = list inst
 
@@ -30,36 +26,27 @@ let rec size : inst -> pos = function
   | Const _ _  -> 1
   | If0 _ i j -> 1 + size_l i + size_l j
   | Seq i -> 1 + size_l i
-
 and size_l : prog -> pos = function
   | [] -> 1
   | hd::tl -> size hd + size_l tl
   
-val override : reg -> rval -> regmap -> regmap
-let override r v rm =
-    fun r' ->
-        if r = r'
-        then v
-        else rm r'
-
 let rec eval' (i:inst) (rm:regmap)
     : Tot regmap (decreases (size i))
     = match i with
-      | Add r1 r2 r3 -> override r3 (rm r1 + rm r2) rm
-      | Sub r1 r2 r3 -> override r3 (rm r1 - rm r2) rm
-      | Mul r1 r2 r3 -> override r3 (rm r1 * rm r2) rm
-      | Const v r    -> override r v rm
+      | Add r1 r2 r3 -> R.upd rm r3 (R.sel rm r1 + R.sel rm r2)
+      | Sub r1 r2 r3 -> R.upd rm r3 (R.sel rm r1 - R.sel rm r2)
+      | Mul r1 r2 r3 -> R.upd rm r3 (R.sel rm r1 * R.sel rm r2)
+      | Const v r    -> R.upd rm r v
       | Seq []       -> rm
       | Seq (p::ps)   -> eval' (Seq ps) (eval' p rm)
       | If0 r p0 p1  ->
-          if rm r = 0 
+          if R.sel rm r = 0 
           then eval' (Seq p0) rm
           else eval' (Seq p1) rm
 
 (* Run in all zeros and get the 0th reg *)
 val eval : prog -> rval
-let eval p = let rm = eval' (Seq p) (fun _ -> 0) in rm (R 0)
-let equiv p1 p2 = eval p1 == eval p2
+let eval p = let rm = eval' (Seq p) (R.create 0) in R.sel rm 0
 
 irreducible
 let unfold_defs = ()
@@ -69,67 +56,109 @@ let normal #a (e:a) =
   FStar.Pervasives.norm 
            [zeta;
             iota;
-            delta_only [`%eval; `%eval'; `%override]; 
+            delta_only [`%eval; `%eval'; `%R.upd; `%R.sel; `%R.eta_map; `%L.append; `%FStar.Mul.op_Star]; 
             delta_attr unfold_defs; 
             primops// ;
             // nbe
   ] e
 
-unfold
-let equiv_norm p1 p2 = normal (eval p1) == normal (eval p2)
+let norm_assert (p:Type) : Lemma (requires (normal p)) (ensures p) = ()
 
 [@unfold_defs]
-let mk42 : prog = [
-    Const 1 (R 0);
-    Add (R 0) (R 0) (R 1);
-    Add (R 1) (R 1) (R 0);
-    Add (R 0) (R 0) (R 1);
-    Add (R 1) (R 1) (R 0);
-    Add (R 0) (R 0) (R 1);
-    Add (R 1) (R 0) (R 0);
-    Const 6 (R 1);
-    Sub (R 0) (R 1) (R 0);
-]
+let reg x = x
 
-let _ = assert_norm (eval mk42 == 42)
+let equiv p1 p2 =
+  (forall rm. 
+     let rm = R.eta_map 10 rm in
+     forall (r:reg_t). R.sel (eval' (Seq p1) rm) r 
+               == R.sel (eval' (Seq p2) rm) r)
 
+[@unfold_defs]
+let all_equiv (rm1 rm2:regmap) =
+    let rec aux (r:reg_t) =
+      R.sel rm1 r == R.sel rm2 r /\
+      (if r = 0 then True
+       else aux (r - 1))
+    in
+    aux 10
+
+[@unfold_defs]
+let equiv_norm p1 p2 =
+    (forall rm. 
+     let rm = R.eta_map 10 rm in
+     all_equiv (eval' (Seq p1) rm)
+               (eval' (Seq p2) rm))
+
+////////////////////////////////////////////////////////////////////////////////
+// Sample programs
+////////////////////////////////////////////////////////////////////////////////
 [@unfold_defs]
 let add1 x y : prog = [
-    Const x (R 0);
-    Const y (R 1);
-    Add (R 0) (R 1) (R 0);
+    Const x (reg 0);
+    Const y (reg 1);
+    Add (reg 0) (reg 1) (reg 0);
 ]
 
 [@unfold_defs]
 let add2 x y : prog = [
-    Const y (R 1);
-    Const x (R 0);
-    Add (R 0) (R 1) (R 0);
+    Const y (reg 1);
+    Const x (reg 0);
+    Add (reg 0) (reg 1) (reg 0);
 ]
     
 [@unfold_defs]
 let add3 x y : prog = [
-    Const x (R 0);
-    Const y (R 1);
-    Add (R 1) (R 0) (R 0);
+    Const x (reg 0);
+    Const y (reg 1);
+    Add (reg 1) (reg 0) (reg 0);
 ]
     
 [@unfold_defs]
 let add4 x y : prog = [
-    Const y (R 1);
-    Const x (R 0);
-    Add (R 1) (R 0) (R 0);
+    Const y (reg 1);
+    Const x (reg 0);
+    Add (reg 1) (reg 0) (reg 0);
 ]
 
-(* All of these identies are quite easy by normalization. Once we fix
- * #1482, they will not even require SMT. *)
-#set-options "--max_fuel 0"
-let _ = assert (forall x y. equiv_norm (add1 x y) (add2 x y))
-let _ = assert (forall x y. equiv_norm (add1 x y) (add3 x y))
-let _ = assert (forall x y. equiv_norm (add1 x y) (add4 x y))
-let _ = assert (forall x y. equiv_norm (add2 x y) (add3 x y))
-let _ = assert (forall x y. equiv_norm (add2 x y) (add4 x y))
-let _ = assert (forall x y. equiv_norm (add3 x y) (add4 x y))
+[@unfold_defs]
+let x_times_42 x : prog = [
+    Const x (reg 0);
+    Add (reg 0) (reg 0) (reg 1); //2x
+    Add (reg 1) (reg 1) (reg 0); //4x
+    Add (reg 0) (reg 0) (reg 1); //8x
+    Add (reg 1) (reg 1) (reg 0); //16x
+    Add (reg 0) (reg 0) (reg 1); //32x
+    Add (reg 1) (reg 0) (reg 0); //48x
+    Const 6 (reg 1);
+    Const x (reg 2);             
+    Mul (reg 1) (reg 2) (reg 1); //6x
+    Sub (reg 0) (reg 1) (reg 0); //42x
+]
+
+[@unfold_defs]
+let long_zero x : prog =
+    let l = x_times_42 x in
+    let l = l `L.append` l in
+    let l = l `L.append` l in
+    let l = l `L.append` l in
+    let l = l `L.append` l in
+    let l = l `L.append` l in    
+    l `L.append` 
+    [Const 0 (reg 0); Const 0 (reg 1); Const 0 (reg 2)]
+
+#set-options "--log_queries --debug Imp --debug_level SMTQuery --debug_level print_normalized_terms"
+let _ = norm_assert (forall x y. equiv_norm (long_zero x) (long_zero y))
+#reset-options "--max_fuel 0"
+let _ = norm_assert (forall x. eval (x_times_42 x) == 42 * x)
+
+
+(* All of these identies are quite easy by normalization. *)
+let _ = norm_assert (forall x y. equiv_norm (add1 x y) (add2 x y))
+let _ = norm_assert (forall x y. equiv_norm (add1 x y) (add3 x y))
+let _ = norm_assert (forall x y. equiv_norm (add1 x y) (add4 x y))
+let _ = norm_assert (forall x y. equiv_norm (add2 x y) (add3 x y))
+let _ = norm_assert (forall x y. equiv_norm (add2 x y) (add4 x y))
+let _ = norm_assert (forall x y. equiv_norm (add3 x y) (add4 x y))
 
 
 (* Without normalizing, they require fuel, or else fail *)
@@ -144,25 +173,25 @@ let _ = assert (forall x y. equiv_norm (add3 x y) (add4 x y))
 
 [@unfold_defs]
 let poly5 x : prog = [
-    Const 1 (R 0);
-    Const x (R 1);
-    Mul (R 1) (R 1) (R 2);
-    Mul (R 1) (R 2) (R 3);
-    Mul (R 1) (R 3) (R 4);
-    Mul (R 1) (R 4) (R 5);
-    Add (R 0) (R 1) (R 0);
-    Add (R 0) (R 2) (R 0);
-    Add (R 0) (R 3) (R 0);
-    Add (R 0) (R 4) (R 0);
-    Add (R 0) (R 5) (R 0);
+    Const 1 (reg 0);
+    Const x (reg 1);
+    Mul (reg 1) (reg 1) (reg 2);
+    Mul (reg 1) (reg 2) (reg 3);
+    Mul (reg 1) (reg 3) (reg 4);
+    Mul (reg 1) (reg 4) (reg 5);
+    Add (reg 0) (reg 1) (reg 0);
+    Add (reg 0) (reg 2) (reg 0);
+    Add (reg 0) (reg 3) (reg 0);
+    Add (reg 0) (reg 4) (reg 0);
+    Add (reg 0) (reg 5) (reg 0);
 ]
 
-let _ = assert (normal (eval (poly5 1)) == 6)
-let _ = assert (normal (eval (poly5 2)) == 63)
-let _ = assert (normal (eval (poly5 3)) == 3*3*3*3*3 + 3*3*3*3 + 3*3*3 + 3*3 + 3 + 1)
+let _ = norm_assert (eval (poly5 1) == 6)
+let _ = norm_assert (eval (poly5 2) == 63)
+let _ = norm_assert (eval (poly5 3) == 3*3*3*3*3 + 3*3*3*3 + 3*3*3 + 3*3 + 3 + 1)
 
 (* Bunch of fuel to even prove ground facts *)
-#reset-options "--initial_fuel 100 --max_fuel 100"
+#reset-options "--initial_fuel 20 --max_fuel 20"
 let _ = assert (eval (poly5 1) == 6)
 let _ = assert (eval (poly5 2) == 63)
 let _ = assert (eval (poly5 3) == 3*3*3*3*3 + 3*3*3*3 + 3*3*3 + 3*3 + 3 + 1)
@@ -171,33 +200,40 @@ let _ = assert (eval (poly5 3) == 3*3*3*3*3 + 3*3*3*3 + 3*3*3 + 3*3 + 3 + 1)
 (* A different way of computing it *)
 [@unfold_defs]
 let poly5' x : prog = [
-    Const 1 (R 0);
-    Const x (R 1);
-    Const 1 (R 2);
-    Mul (R 0) (R 1) (R 0);
-    Add (R 0) (R 2) (R 0);
-    Mul (R 0) (R 1) (R 0);
-    Add (R 0) (R 2) (R 0);
-    Mul (R 0) (R 1) (R 0);
-    Add (R 0) (R 2) (R 0);
-    Mul (R 0) (R 1) (R 0);
-    Add (R 0) (R 2) (R 0);
-    Mul (R 0) (R 1) (R 0);
-    Add (R 0) (R 2) (R 0);
+    Const 1 (reg 0);
+    Const x (reg 1);
+    Const 1 (reg 2);
+    Mul (reg 0) (reg 1) (reg 0);
+    Add (reg 0) (reg 2) (reg 0);
+    Mul (reg 0) (reg 1) (reg 0);
+    Add (reg 0) (reg 2) (reg 0);
+    Mul (reg 0) (reg 1) (reg 0);
+    Add (reg 0) (reg 2) (reg 0);
+    Mul (reg 0) (reg 1) (reg 0);
+    Add (reg 0) (reg 2) (reg 0);
+    Mul (reg 0) (reg 1) (reg 0);
+    Add (reg 0) (reg 2) (reg 0);
 ]
 
 (* Seems to do the same *)
-let _ = assert (normal (eval (poly5' 1)) == 6)
-let _ = assert (normal (eval (poly5' 2)) == 63)
-let _ = assert (normal (eval (poly5' 3)) == 3*3*3*3*3 + 3*3*3*3 + 3*3*3 + 3*3 + 3 + 1)
+let _ = norm_assert (eval (poly5' 1) == 6)
+let _ = norm_assert (eval (poly5' 2) == 63)
+let _ = norm_assert (eval (poly5' 3) == 3*3*3*3*3 + 3*3*3*3 + 3*3*3 + 3*3 + 3 + 1)
+let _ = norm_assert (forall x. eval (poly5 x) == eval (poly5' x))
 
 (* Same *)
-#reset-options "--initial_fuel 100 --max_fuel 100"
+#reset-options "--initial_fuel 20 --max_fuel 20"
 let _ = assert (eval (poly5' 1) == 6)
 let _ = assert (eval (poly5' 2) == 63)
 let _ = assert (eval (poly5' 3) == 3*3*3*3*3 + 3*3*3*3 + 3*3*3 + 3*3 + 3 + 1)
-let _ = assert (forall x. poly5 x `equiv` poly5' x)
+let _ = assert (forall x. (eval (poly5 x) == eval (poly5' x)))
 #reset-options "--max_fuel 0"
+
+//--------------------------------------------------------------------------------
+
+// open FStar.Tactics
+// open CanonCommSemiring
+// open FStar.Algebra.CommMonoid
 
 // [@Pervasives.fail]
 // let _ = assert (forall x. poly5 x `equiv` poly5' x)
